\\\\a)(2x+3)^2=(2x)^2+2\cdot2x\cdot3+3^2=4x^2+12x+9
\\\\b)(2a^2-3)^2=(2a^2)^2-2\cdot2a^2\cdot3+3^2=4a^4-12a^2+9
\\\\c)4ax-8ay=4a(x-2y)
\\\\d)\dfrac{x^2+xy}{2x}=\dfrac{\cancel x(x+y)}{2\cancel x}=\dfrac{x+y}2
\\\\e)4xy^2+16x^4y^3-12x^2y=4xy(y+4x^3y^2-3x)
\\\\f)2x+5xy+y=2x+y(5x+1)
\\\\g)2x+3(3-2x)-2(1-x)=2x+9-6x-2+2x=-2x+7
\\\\h)3(a^2+a+1)+2(a^2+2a-2)-(a^2+3a-3)=
\\3a^2+3a+3+2a^2+4a-4-a^2-3a+3=
\\4a^2+4a+2=2(2a^2+2a+1)
\\\\i)x(x^2-xy+y^2)+y(x^2-xy+y^2)=x^3\cancel{-x^2y}+\cancel{xy^2}+\cancel{x^2y}-\cancel{xy^2}+y^3=x^3+y^3